clean up

src/Common.fst
@@ -25,7 +25,31 @@ module M   = LowStar.Modifies
 module HS  = FStar.HyperStack
 module HST = FStar.HyperStack.ST
 
-let ret_TRUE  : int32 = i32 1
-let ret_FALSE : int32 = i32 0
-let ret_ERROR : int32 = i32 (-1)
+let ret_SUCCESS : int32 = i32 1
+let ret_FAILURE : int32 = i32 0
+let ret_ERROR   : int32 = i32 (-1)
 
+let _DICE_UDS_LENGTH = 0x20
+
+assume val uds : B.lbuffer uint8 _DICE_UDS_LENGTH
+
+type imagePath =
+
+noeq
+type hinstance = {
+     addr: B.pointer uint32
+  }
+
+assume val _DEFAULT_RIOT_PATH: B.buffer imagePath
+assume val _DEFAULT_LOADER_PATH: B.buffer imagePath
+
+
+noeq
+type cdi_t = {
+     alg: hash_alg;
+     cdi: hash_t alg;
+  }
+
+
+type entryPoint =
+assume val _RIOT_ENTRY: entryPoint
